theories/rules/halt.v
@@ -15,17 +15,21 @@ Lemma halt {E i w1 q s} ai :
           ∗ ▷ (ai ->a w1)
           ∗ ▷ (A@i:={q}[s])}}}
     ExecI @ i ;E
- {{{ RET HaltI;  PC @@ i ->r (ai ^+ 1)%f
+ {{{ RET (false, HaltI);  PC @@ i ->r (ai ^+ 1)%f
                   ∗ ai ->a w1
                   ∗ A@i:={q}[s] }}}.
 Proof.
   iIntros (Hdecode Hin ϕ) "(>Hpc & >Hapc & >Hacc) Hϕ".
   iApply (sswp_lift_atomic_step ExecI);[done|].
-  iIntros (σ1) "%Hsche Hσ".
-  inversion Hsche as [ Hcur ]; clear Hsche.
+  iIntros (n σ1) "%Hsche Hσ".
+  rewrite /scheduled in Hsche.
+  simpl in Hsche.
+  rewrite /scheduler in Hsche.
+  apply bool_decide_unpack in Hsche as Hcur.
+  clear Hsche.
   apply fin_to_nat_inj in Hcur.
   iModIntro.
-  iDestruct "Hσ" as "(Htok & Hmem & Hreg & Htx & Hrx1 & Hrx2 & Hown & Haccess & Hrest)".
+  iDestruct "Hσ" as "(#Hneq & Hmem & Hreg & Htx & Hrx1 & Hrx2 & Hown & Haccess & Hrest)".
   (* valid regs *)
   iDestruct ((gen_reg_valid1 PC i ai Hcur ) with "Hreg Hpc") as "%HPC";eauto.
   (* valid pt *)
@@ -38,7 +42,7 @@ Proof.
     apply (reducible_normal i Halt ai w1);eauto.
   - (* step *)
     iModIntro.
-    iIntros (m2 σ2) "%HstepP".
+    iIntros (m2 σ2) "[%P PAuth] %HstepP".
     apply (step_ExecI_normal i Halt ai w1 ) in HstepP;eauto.
     remember (exec Halt σ1) as c2 eqn:Heqc2.
     rewrite /exec /halt /update_incr_PC in Heqc2;eauto.
@@ -47,15 +51,36 @@ Proof.
     (* unchanged part *)
     rewrite_reg_pc.
     rewrite_reg_global.
-    rewrite Hcur.
-    iFrame "Htok Hmem Htx Hrx1 Hrx2 Hown Haccess Hrest".
+    iFrame "Hmem Htx Hrx1 Hrx2 Hown Haccess Hrest".
     (* updated part *)
     iDestruct ((gen_reg_update1_global PC i ai (ai ^+ 1)%f) with "Hreg Hpc") as ">[Hreg Hpc]";eauto.
     rewrite -> (update_offset_PC_update_PC1 _ i ai 1);eauto.
     iModIntro.
     iFrame "Hreg".
+    iSplitL "PAuth".
+    iExists P.
+    iFrame.
+    iSplit; first done.
+    rewrite /just_scheduled_vms.
+    rewrite /just_scheduled.
+    assert (filter
+              (λ id : vmid,
+                      base.negb (scheduled σ1 id) && scheduled (update_offset_PC σ1 1) id = true)
+              (seq 0 n) = []) as ->.
+    admit.
+    iSimpl.
+    iSplit; first done.
+    assert ((scheduled (update_offset_PC σ1 1) i) = true) as ->.
+    rewrite /scheduled.
+    simpl.
+    rewrite /scheduler.
+    rewrite update_offset_PC_preserve_current_vm.
+    rewrite Hcur.
+    rewrite bool_decide_eq_true.
+    reflexivity.
+    simpl.
     iApply "Hϕ".
     by iFrame "Hpc Hapc Hacc".
     apply (get_reg_gmap_get_reg_Some _ _ _ i) in HPC;eauto.
-Qed.
+Admitted.
 End halt.
