theories/rules/run.v
@@ -1,6 +1,6 @@
 From machine_program_logic.program_logic Require Import weakestpre.
 From HypVeri Require Import lifting rules.rules_base.
-From HypVeri.algebra Require Import base reg mem token pagetable.
+From HypVeri.algebra Require Import base reg mem pagetable.
 From HypVeri.lang Require Import lang_extra reg_extra current_extra.
 Require Import stdpp.fin.
 
@@ -15,27 +15,30 @@ Lemma run {z w1 w2 w3 q s E} ai i :
   fin_to_nat z = 0 -> 
   decode_hvc_func w2 = Some Run ->
   decode_vmid w3 = Some i ->
-  {SS{{ ▷ (<<z>>{ 1%Qp })
-          ∗ ▷ (PC @@ z ->r ai)
+  {SS{{ ▷ (PC @@ z ->r ai)
           ∗ ▷ (ai ->a w1)
           ∗ ▷ (A@z :={q}[s] )
           ∗ ▷ (R0 @@ z ->r w2)
-          ∗ ▷ (R1 @@ z ->r w3)}}}
+          ∗ ▷ (R1 @@ z ->r w3)
+          ∗ ▷ (VMProp_holds i)}}}
     ExecI @ z ;E
-    {{{ RET ExecI; <<i>>{ 1%Qp }
-                     ∗ PC @@ z ->r (ai ^+ 1)%f
+    {{{ RET (true, ExecI); PC @@ z ->r (ai ^+ 1)%f
                      ∗ ai ->a w1
                      ∗ A@z :={q}[s]
                      ∗ R0 @@ z ->r w2
                      ∗ R1 @@ z ->r w3 }}}.
 Proof.
-  iIntros (Hdecode Hin Hz Hhvc Hvmid ϕ) "(>Htok & >Hpc & >Hapc & >Hacc & >Hr0 & >Hr1) Hϕ".
+  iIntros (Hdecode Hin Hz Hhvc Hvmid ϕ) "(>Hpc & >Hapc & >Hacc & >Hr0 & >Hr1 & HProp) Hϕ".
   iApply (sswp_lift_atomic_step ExecI); [done|].
-  iIntros (σ1) "%Hsche Hσ".
-  inversion Hsche as [ Hcur ]; clear Hsche.
+  iIntros (n σ1) "%Hsche Hσ".
+  rewrite /scheduled in Hsche.
+  simpl in Hsche.
+  rewrite /scheduler in Hsche.
+  apply bool_decide_unpack in Hsche as Hcur.
+  clear Hsche.
   apply fin_to_nat_inj in Hcur.
   iModIntro.
-  iDestruct "Hσ" as "(Htokown & Hmemown & Hregown & Htx & Hrx1 & Hrx2 & Hown & Haccessown & Hrest)".
+  iDestruct "Hσ" as "(%Hneq & Hmemown & Hregown & Htx & Hrx1 & Hrx2 & Hown & Haccessown & Hrest)".
   (* valid regs *)
   iDestruct (gen_reg_valid1 PC z ai Hcur with "Hregown Hpc") as "%Hpc".
   iDestruct (gen_reg_valid1 R0 z w2 Hcur with "Hregown Hr0") as "%Hr0".
@@ -49,8 +52,8 @@ Proof.
     iPureIntro.
     apply (reducible_normal z Hvc ai w1);eauto.
   - iModIntro.
-    iIntros (m2 σ2 Hstep).
-    apply (step_ExecI_normal z Hvc ai w1) in Hstep; eauto.
+    iIntros (m2 σ2) "[%P PAuth] %HstepP".
+    apply (step_ExecI_normal z Hvc ai w1) in HstepP; eauto.
     remember (exec Hvc σ1) as c2 eqn:Heqc2.
     rewrite /exec /hvc in Heqc2; eauto.
     rewrite  Hr0 Hhvc /run Hr1 in Heqc2.
@@ -59,28 +62,38 @@ Proof.
     simpl in Heqc2.
     rewrite /is_primary Hcur Hz in Heqc2.
     destruct (0 =? 0) eqn:Hvmz; [|done].
-    destruct Hstep as [Hstep1 Hstep2].
+    destruct HstepP as [Hstep1 Hstep2].
     simplify_eq.
     simpl.
     rewrite /gen_vm_interp /update_incr_PC.
     rewrite_vmid_all.
     rewrite_reg_pc.
-    iFrame "Hrest Htx Hrx1 Hrx2 Hmemown Haccessown".
+    iFrame "Hrest Htx Hrx1 Hrx2 Hmemown Haccessown Hown".
     iDestruct ((gen_reg_update1_global PC (get_current_vm σ1) ai (ai ^+ 1)%f) with "Hregown Hpc") as "HpcUpd".
-    iDestruct (token_update (get_current_vm σ1) (get_current_vm σ1) i with "Htok") as "HtokUpd".
-    rewrite token_agree_eq /token_agree_def.
-    iDestruct ("HtokUpd" with "Htokown") as "Htok'". 
-    rewrite /get_current_vm /update_current_vmid.
-    simpl.
     rewrite ->(update_offset_PC_update_PC1 _ (get_current_vm σ1) ai 1); auto.
     + iMod "HpcUpd".
-      iMod "Htok'".
       iModIntro.
-      iDestruct "Htok'" as "[Htok1 Htok2]".
       iDestruct "HpcUpd" as "[? ?]".
       iFrame.
+      iSplitL "PAuth".
+      iExists P.
+      iFrame.
+      iSplit; first done.
+      iSplitL "HProp".
+      rewrite /just_scheduled_vms /just_scheduled.
+      assert (filter
+                (λ id : vmid,
+                        base.negb (scheduled σ1 id) &&
+                        scheduled (update_current_vmid (update_offset_PC σ1 1) i) id = true)
+                (seq 0 vm_count) = [fin_to_nat i]) as ->.
+      admit.
+      iSimpl.
+      iSplit; last done.
+      iFrame.
+      assert ((negb (scheduled (update_current_vmid (update_offset_PC σ1 1) i) (get_current_vm σ1)) && true = true)) as ->.
+      admit.
       iApply "Hϕ".
       by iFrame.
     + apply get_reg_gmap_get_reg_Some; auto.
-Qed.
+Admitted.
 End run.
